Prove that m in REDC is correct

montgomery-correctness.ec
@@ -5,23 +5,16 @@ from Jasmin require import JModel.
 op dilithium_modulo = 8380417.
 op dilithium_modulo_left_shift41 = 18428731874223325184.
 op dilithium_modulo_inv = 58728449.
-
-(*
-lemma dilithium_mod_right_inv_correct:
-    dilithium_modulo * dilithium_modulo_inv %% (2 ^ 32) = 1.
-proof.
-    trivial.
-qed.
-
-lemma dilithium_mod_left_inv_correct:
-    dilithium_modulo_inv * dilithium_modulo %% (2 ^ 32) = 1.
-proof.
-    trivial.
-qed.
-  *)
+op dilithium_modulo_minus_inv = 4236238847.
 
 lemma dilithium_mod_inv_correct:
     dilithium_modulo_inv * dilithium_modulo %% (2 ^ 32) = 1.
+proof.
+    trivial.
+qed.
+
+lemma dilithium_mod_minus_inv_correct:
+    dilithium_modulo_minus_inv = (-dilithium_modulo_inv) %% (2 ^ 32).
 proof.
     trivial.
 qed.
@@ -39,6 +32,76 @@ op montgomery_redc = fun (a' : int) =>
     let m = montgomery_redc_m(a') in
     let t = montgomery_redc_t(a') in
     if t < dilithium_modulo then t else t - dilithium_modulo.
+
+lemma W64_AND_mod32 x:
+    (W64.of_int x) `&` (W64.of_int 4294967295) = W64.of_int (x %% 4294967296).
+proof.
+    have twoTo32: 4294967295 = 2 ^ 32 - 1 by trivial.
+    rewrite twoTo32.
+    rewrite and_mod.
+    trivial.
+    rewrite of_uintK.
+    rewrite modz_dvd.
+    simplify.
+    auto.
+    simplify.
+    trivial.
+qed.
+
+(*
+
+lemma and_mod32 x: 
+    x `&` W64.of_int 4294967295 = W64.of_int (to_uint x %% 4294967296).
+proof.
+    have twoTo32: 4294967295 = 2 ^ 32 - 1 by trivial.
+    rewrite twoTo32.
+    rewrite and_mod.
+    simplify.
+    trivial.
+    simplify.
+    done.
+qed.
+    *)
+
+lemma montgomery_redc_impl_correct:
+    forall x_, 0 <= x_ < dilithium_modulo =>
+    hoare[M.montgomery_REDC : x = W64.of_int x_ ==> res = W64.of_int (montgomery_redc x_)].
+proof.
+    move => x_.
+    case.
+    move => x_lower_bound x_upper_bound.
+    proc.
+    seq 4 : (x = (of_int x_) % W64 /\ m = W64.of_int (montgomery_redc_m x_)).
+    sp.
+    skip.
+    rewrite andbC.
+    move => &hr.
+    case.
+    move => xhr_def mhr_def.
+    rewrite xhr_def in mhr_def.
+    rewrite W64_AND_mod32 in mhr_def.
+    rewrite pmod_small in mhr_def.
+    split.
+    apply x_lower_bound.
+    move => unused.
+    have mod_lt_2to32: dilithium_modulo < 4294967296 by trivial.
+    (* Using smt since I somehow can't get transitivity to work... *)
+    (* datatypes/Int.ec *)
+    (* 47 axiom nosmt ltz_trans : forall y x z, x < y => y < z => x < z. *)
+    smt.
+    split.
+    apply xhr_def.
+    rewrite W64.of_intM' in mhr_def.
+    rewrite - /dilithium_modulo_minus_inv in mhr_def.
+    rewrite dilithium_mod_minus_inv_correct in mhr_def.
+    rewrite W64_AND_mod32 in mhr_def.
+    rewrite /montgomery_redc_m.
+    rewrite modzMmr in mhr_def.
+    (* Minus signs and stuff... *)
+    smt.
+
+
+    
 
 lemma montgomery_correct_div_t:
     forall a', 0 <= a' < dilithium_modulo =>
@@ -66,51 +129,8 @@ proof.
     simplify.
 done.
 
-(*
-251 (* -------------------------------------------------------------------- *)
-252 lemma nosmt modzE m d : m %% d = m - (m %/ d) * d.
-253 proof. by have [+ _] - {2}-> := edivzP m d; rewrite addrAC addrN. qed.
-254
-255 (* -------------------------------------------------------------------- *)
-256 lemma nosmt divzE m d : m %/ d * d = m - m %% d.
-257 proof. by rewrite modzE; ring. qed.
-*)
-    
-
-    
-            
-    
 
 
-
-        
-
-
-
-
-
-(* Add-linear?
-Want: (a%d + b%d) %d = (a+b)%d
-*)
-
-(*
-337 lemma nosmt modzDml m n d : (m %% d + n) %% d = (m + n) %% d.
-338 proof. by rewrite {2}(divz_eq m d) -addrA modzMDl. qed.
-339
-340 lemma nosmt modzDmr m n d : (m + n %% d) %% d = (m + n) %% d.
-341 proof. by rewrite !(addrC m) modzDml. qed.
-*)
-
-(* mult-linear: modzMml *)
-(* modzMml m n d : ((m %% d) * n) %% d = (m * n) %% d *)
-    
-
-    
-    
-
-
-
-    
 
 
 lemma montgomery_redc_is_left_inv:
